Milestones.thy
@@ -1,0 +1,43 @@
+theory Milestones
+imports Main Running_Example
+begin
+
+section \<open>Minimum Viable Product\<close>
+
+text \<open>13.12.24: Normalization\<close>
+
+lemma "ast_problem.valid_plan P \<pi> \<Longrightarrow> ast_problem.valid_plan (detype_prob P) \<pi>"
+  oops
+
+text \<open>20.12.24: Relaxed Reachability \<close>
+
+lemma
+  assumes "ast_problem.wf_problem P"
+          "ast_problem.plan_action_path P (set (init P)) \<pi>s s'"
+          "s' \<^sup>c\<TTurnstile>\<^sub>= Atom (predAtm prd params)"
+  obtains s'' where
+    "ast_problem.plan_action_path (relax_prob P) (set (init (relax_prob P))) \<pi>s s''"
+    "s'' \<^sup>c\<TTurnstile>\<^sub>= Atom (predAtm prd params)"
+
+text \<open>27.12.24: Datalog translation\<close>
+
+
+section \<open>Helmert's Rule Decomposition\<close>
+
+
+
+
+section \<open>Tree Decomposition\<close>
+
+
+
+section \<open>"iterated"\<close>
+
+
+
+
+
+
+
+
+end
