Documentation/knowledge.md
@@ -12,6 +12,7 @@
 - "flat type hierarchy"?
 
 **Orga**
+- Scope: What's the minimum to pass? And what would give me my desired grade?
 - Can this project become part of the AFP? What would I need to watch out for? Can something be in AFP with external dependencies (Datalog formalization is not in AFP)?
 # Dependencies (tentative):
 - [NetworkX](https://networkx.org/documentation/stable/reference/algorithms/generated/networkx.algorithms.approximation.treewidth.treewidth_min_degree.html) (python library):
@@ -24,7 +25,7 @@
 - [Ab+Ku] Abdulaziz, Kurz 2020: [Verified SAT-Based AI Planning ](https://www.isa-afp.org/entries/Verified_SAT_Based_AI_Planning.html) 
 	- Includes Isabelle formalization of propositional STRIPS
 	- output format of application
-	- Paper: ([link](https://kclpure.kcl.ac.uk/ws/portalfiles/portal/189846427/verified_SAT_plan.pdf))
+	- Paper: ([link](https://arxiv.org/pdf/2010.14648))
 - Schlichtkrull et al 2024: [Isabelle-verified correctness of Datalog programs for program analysis](https://github.com/anderssch/LTS-formalization)
 	- Isabelle formalization of Datalog semantics and verifier, but not solver.
 	- Paper: ([link](https://people.cs.aau.dk/~andsch/SAC2024.pdf))
@@ -58,9 +59,11 @@
 
 # Citation Needed
 - For every clique, in any tree decomposition, there exists a bag where clique $\subseteq$ bag. Thus, the variable set of any rule can be assigned to a bag.
+	- [Stackexchange](https://math.stackexchange.com/questions/1227867/a-clique-in-a-tree-decomposition-is-contained-in-a-bag)
 
 
 # Source Notes
+- "lifted" $\leftrightarrow$ "grounded"
 ## Main Sources
 ### <ins>Helmert</ins>
 - [ ] detailed dissection currently at **6. Grounding**
@@ -102,27 +105,58 @@
 - For preconditions, turn formula into CNF then split into multiple operators across disjunctions. **NNF may be enough due to properties of STRIPS formulas, then no need to split operators.**
 
 **Datalog generation**
+- Datalog is declarative programming language for logic
 - straight forward. $\mathit{A\\\_applicable}(\cdot)\leftarrow\mathit{A\\\_pre}(\cdot)$
-$\mathit{A\\\_effects}(\cdot)\leftarrow\mathit{A\\\_applicable}(\cdot)$
+$\mathit{A\\\_effect_i}(\cdot)\leftarrow\mathit{A\\\_applicable}(\cdot)$
+- How can you ensure that this is "safe"? What if my action just doesn't have preconditions? Can you have an (implicit) $\forall$-quantifier in the head?
+	- Rules are never unsafe here, because you always have type-preconditions for every variable. If the reader wants to build this for un-typed PDDL, they can add $\mathit{dummy}(x)$ in the body where needed. The dummy predicate is contained in the facts for every constant.
+	- Alternative: $H(x, y)\leftarrow P(x)$ is illegal, so you might do
+$H_{\forall2}(x)\leftarrow P(x)$ and then add many rules
+$H(x, y_k) \leftarrow H_{\forall2}(x)$
 
 **Datalog rule decomposition**
-* Join decomposition: If $q_1(\cdot), q_2(\cdot)\in\mathit{body}$, create new predicate with rule $\mathit{temp}(\cdot)\leftarrow q_1(\cdot), q_2(\cdot)$.
-* Projection: Find an atom $q$ in a body that uses a variable $v$ unused elsewhere in the rule, then add $\mathit{temp}(\cdot\backslash v)\leftarrow q(\cdot)$. This reduces variable count by essentially resolving existential qualifiers. E.g.: $Q(\mathit{room})\leftarrow\mathit{holding}(\mathit{box}),\mathit{at}(\mathit{room})$ is simplified by introducing $\mathit{holding\\\_any\\\_box}()\leftarrow\mathit{holding}(\mathit{box})$
-* Problem: how to choose joins. Helmert chooses atoms with many variables.
+- Definition 14: I can probably explain this a little more elaborately.
+- ...
+- Problem: how to choose joins. Helmert chooses atoms with many variables (**TODO** find quote. This is a claim by Correa).
 
 ### <ins>Correa</ins>
 - [x] fully dissected
-- (**double check**) Can ground more problems in total because of good space efficiency, but is comparatively time inefficient.
+- (**double check**) Can ground more problems in total because of good space efficiency, but is comparatively time inefficient due to overhead.
 - Iterated<sup>≠</sup> is confusing...
-- TODO copy rest of my notes here
+- Grounding simplifies a problem from first-order logic to propositional logic.
 
-**Rule Decomposition**
+**PDDL stuff**
+- $\neq$ treated as static built-in predicate by e.g. gringo (also by Ab+La)
+
+**Logic Programs**
+- More general: *Answer Set Programming* (ASP)
+- More restrictive: *I think* Stratified Datalog. Only allows single atom in head.
+- More restrictive: Datalog. Doesn't allow negative atoms.
+- Logic program $\mathcal L =\langle\mathcal F, \mathcal R\rangle$
+	- $\mathcal F$: facts
+	- $\mathcal R$: set of disjunctive rules like
+$r:=\underbrace{H_1 \lor \dots\lor H_k}_{\mathit{head(r)}}\leftarrow\underbrace{P_1, \dots, P_n}_{\mathit{body}^{+}(r)}, \underbrace{\neg N_1, \dots, \neg N_m}_{\mathit{body}^{-}(r)}$
+	- "All rules we considered are safe"? I.e. $\mathit{free}(\mathit{head}(r))\subseteq \mathit{free}(\mathit{body}(r))$. Otherwise, too many atoms would follow from one body instantiation.
+	- Atoms can have a mix of constants and variables. $\mathcal F$ contains ground atoms only.
+	- A stable model $\mathcal M$ is a solution and satisfies each fact and each rule. (And all facts, aside from the initial facts, are derived from rules.)
+- "each Datalog program has a unique stable model M, called the *canonical model*". Can be iteratively constructed from $\mathcal F$. **TODO this doesn't apply to stratified Datalog, right?**
+
+**Datalog Translation**
+- Add goal rule. If goal isn't reachable, don't even bother grounding the program.
+
+**Simple Rule Decomposition**
 - Simple join/projection decompositions: "different choices on how to decompose rules will lead to a different number of temporary predicates." Correa claims preferring atoms with few variables yields better results, whereas Helmert prefers atoms with many variables (page 3 footnote 2).
-- Can use tree decomposition instead.
+- Join decomposition: If $q_1(\cdot), q_2(\cdot)\in\mathit{body}$, create new predicate with rule $\mathit{temp}(\cdot)\leftarrow q_1(\cdot), q_2(\cdot)$. **Improvement**: If we strictly follow Definition 14 in Helmert, if $v\in\mathit{free}(q_1)\cap\mathit{free}(q_2)$ does not appear elsewhere in the original $\mathit{body}$, then we can omit $v$ from the parameters of $\mathit{temp}$.
+- Projection: Find an atom $q$ in a body that uses a variable $v$ unused elsewhere in the rule, then add $\mathit{temp}(\cdot\backslash v)\leftarrow q(\cdot)$. This reduces variable count by essentially resolving existential qualifiers. E.g.: $Q(\mathit{room})\leftarrow\mathit{holding}(\mathit{box}),\mathit{at}(\mathit{room})$ is simplified by introducing $\mathit{holding\\\_any\\\_box}()\leftarrow\mathit{holding}(\mathit{box})$
+
+**Advanced Rule Decomposition with Tree Decomp**
+- Rule $r$ gets primal graph $G_r=\langle V, E\rangle$ where $V=\mathit{vars}(r), (v_1, v_2)\in E \Leftrightarrow \exists P(t)\in\mathit{head}(r)\cup\mathit{body}(r): v_1, v_2\in\mathit{vars}(t)$. $P$ is a predicate and the terms $t$ the parameters.
+- Tree decompose this graph. Many rules have low tree width, hence efficient grounding if good decomposition is found.
 - lpopt generates "n new rules": Probably a mistake, you need more rules for disjunctions.
+- Tree width can only be 1 (primal graph uncyclic) if every pred in the body has only 2 variables.
 
 **iterated**
-- Avoid grounding actions at first by skilling applicability rules and instead directly feeding into action effect rules ("simplified" problem),
+- Avoid grounding actions at first by skilling applicability rules and instead directly feeding into action effect rules ("simplified" problem). Create a separate rule for each (add) effect.
 - This only immediately generates reachable atoms, not ground actions.
 - Trivial solution: unify preconditions and explode exponentially
 - Actual solution: iterated solving: Solve the simplified problem, obtain solution $\mathcal M$. For every action, create new program with facts $\mathcal F := \mathcal M$ and "choice rules".
@@ -130,6 +164,7 @@ $\mathit{A\\\_effects}(\cdot)\leftarrow\mathit{A\\\_applicable}(\cdot)$
 For non-ground atom $q_i$ in body with variables $V_{\dots k}$ create $\bot\leftarrow \mathit{v_{1}\\\_ assign}(x_1), \dots, \mathit{v_k\\\_assign}(x_k), \neg q_i(x_1, \dots, x_k)$.
 But how can he use negation? Is it not Datalog but ASP/stratified Datalog?
 - Each stable model is then one ground action. Iteratively solve and enumerate all of them.
+- **?**: When removing applicability rules, the result isn't safe necessarily. 
 
 **iterated<sup>≠</sup>**
 - "negated static predicates" why is ≠ negated? It can just be a predicate, why would FD not already consider it in the simplified problem?
@@ -151,6 +186,7 @@ But how can he use negation? Is it not Datalog but ASP/stratified Datalog?
 - `term`: Union of variable and object
 - preconditions and goal formulas can have any structure
 - add overwrites del effects
+- $\neq$ is a type of formula atom. It is essentially a built-in, static predicate.
 
 **Lifschitz Consistency**
 - Definition of system according to Lifschitz 1987, definition "B".
@@ -216,6 +252,21 @@ But how can he use negation? Is it not Datalog but ASP/stratified Datalog?
 	- Ab+La uses Definition B
 
 
-# Explanations (with citations)
+# Explanations
 ### Why consts/objects should have primitive types
 TODO
+
+### Rule Decomposition Examples
+Join decompositions can remove $y$ from head eventually, because $r$ does not contain $y$.
+$r(x, z, w) \leftarrow \underbrace{p(x, y), q(x, y)}_{pq}, s(y, z), t(z, w, v)$
+1. $pq(x, y) \leftarrow p(x, y), q(x, y)$ | valid join rule
+$r(x, z, w) \leftarrow \underbrace{pq(x, y), s(y, z)}_{pqs}, t(z, w, v)$
+2. $pqs(x, z) \leftarrow pq(x, y), s(y, z)$ | valid join rule
+$r(x, z, w) \leftarrow pqs(x, z), \underbrace{t(z, w, v)}_{t_{\exists3}}$
+3. $t_{\exists 3}(z, w)\leftarrow t(z, w, v)$ | valid projection rule
+$r(x, z, w) \leftarrow pqs(x, z), t_{\exists3}(z, w)$ | valid join rule
+
+There's also the concept of variable-uniqueness where variable repetition like $p(x, y, x)$ isn't allowed. **TODO how is that ensured?** Probably by modifying the predicates and facts in a preprocessing step?
+
+**Why relaxed reachability**
+If you allow negative atoms, previously derived atoms could become false in the future.  You would need reassignments, which would greatly complicate the iterative Datalog solver.
